| Expression                     | Fully-Parenthesized Expression         |
|--------------------------------|---------------------------------------|
| `a + b + c`                    | `((a + b) + c)`                       |
| `a = b = c`                    | `(a = (b = c))`                       |
| `c = a + b`                    | `(c = (a + b))`                       |
| `d = a && !b || c`             | `(d = ((a && (!b)) || c))`            |
| `++*p++`                       | `(++(*(p++)))`                        |
| `a | ~b & c ^ d`               | `(a | (((~b) & c) ^ d))`              |
| `a[0]++ + a[1]++`              | `(((a[0])++) + ((a[1])++))`           |
| `a + b * c / d % -g`           | `(a + (((b * c) / d) % (-g)))`        |
| `++p[i]`                       | `(++(p[i]))`                          |
| `--*++p`                       | `(--(*(++p)))`                        |
| `a += b += c += d`             | `(a += (b += (c += d)))`              |
| `z = a == b ? ++c : --d`       | `(z = ((a == b) ? (++c) : (--d)))`    |
| `a + b <=> c + d > 0`          | `((a + b) <=> (c + d)) > 0`           |
